git/siddhartha-gadgil/Polylean/Polylean/MetabelianGroup.lean
@@ -1,5 +1,6 @@
 import Polylean.Morphisms
 import Polylean.GroupAction
+import Polylean.Experiments.Tactics
 
 /-
 Metabelian groups are group extensions `1 → K → G → Q → 1` with both the kernel and the quotient abelian. Such an extension is determined by data:
@@ -66,19 +67,28 @@ variable (c : Q → Q → K) [ccl : Cocycle c]
 The multiplication operation defined using the cocycle.
 The cocycle condition is crucially used in showing associativity and other properties.
 -/
-def mul : (K × Q) → (K × Q) → (K × Q)
+@[reducible] def mul : (K × Q) → (K × Q) → (K × Q)
   | (k, q), (k', q') => (k + (q • k') + c q q', q + q')
 
 def e : K × Q := (0, 0)
 
-def inv : K × Q → K × Q
+@[reducible] def inv : K × Q → K × Q
   | (k, q) => (- ((-q) • (k  + c q (-q))), -q)
 
 theorem left_id : ∀ (g : K × Q), mul c e g = g
   | (k, q) => by simp [e, mul]
 
 theorem right_id : ∀ (g : K × Q), mul c g e = g
-  | (k, q) => by simp [e, mul]
+  | (k, q) => by 
+        rw [e, mul]
+        show (k + q • 0 + c q 0, q + 0) = (k, q)
+        have cq0 : c q 0 = 0 := by apply Cocycle.rightId
+        rw [cq0]
+        have q0 : q • (0 : K) = 0 := 
+          by apply AutAction.act_zero
+        rw[q0]
+        repeat (rw [add_zero])
+
 
 theorem left_inv : ∀ (g : K × Q), mul c (inv c g) g = e
   | (k , q) => by
@@ -123,6 +133,10 @@ instance metabeliangroup : Group (K × Q) :=
     gpow_neg' := by intros; rfl,
   }
 
+def mult (k k' : K) (q q' : Q) : (k, q) * (k', q') =  (k + (q • k') + c q q', q + q') := rfl
+
+def inverse (k : K) (q : Q) : (k, q)⁻¹ = (- ((-q) • (k  + c q (-q))), -q) := rfl
+
 end MetabelianGroup
 
 
@@ -142,7 +156,7 @@ instance G : Group (K × Q) := MetabelianGroup.metabeliangroup c
 
 -- this is the subgroup of the metabelian group that occurs as
 -- the image of the inclusion of `K` and the kernel of the projection onto `Q`.
-def Metabelian.Kernel := subType (λ ((k, q) : K × Q) => q = (0 : Q))
+def Metabelian.Kernel := subType (λ ((_, q) : K × Q) => q = (0 : Q))
 
 def Metabelian.Kernel.inclusion : K → (Metabelian.Kernel Q K)
   | k => ⟨(k, 0), rfl⟩
@@ -150,44 +164,51 @@ def Metabelian.Kernel.inclusion : K → (Metabelian.Kernel Q K)
 def Metabelian.Kernel.projection : (Metabelian.Kernel Q K) → K
   | ⟨(k, _), _⟩ => k
 
-instance : subGroup (λ ((k, q) : K × Q) => q = (0 : Q)) where
+instance : subGroup (λ ((_, q) : K × Q) => q = (0 : Q)) where
   mul_closure := by
-    intro ⟨ka, qa⟩ ⟨kb, qb⟩; intro hqa hqb
-    show (Mul.mul (ka, qa) (kb, qb)).snd = 0
-    simp [Mul.mul, MetabelianGroup.mul] at *
-    rw [hqa, hqb, add_zero]
+    intro ⟨ka, qa⟩ ⟨kb, qb⟩; intro (hqa : qa = 0) (hqb : qb = 0)
+    subst hqa hqb
+    reduceGoal
+    rw [add_zero]
   inv_closure := by
-    intro ⟨ka, qa⟩; intro h
-    simp [Inv.inv, MetabelianGroup.inv] at *
-    apply neg_eq_of_add_eq_zero
-    rw [h, add_zero]
+    intro ⟨ka, qa⟩; intro (h : qa = 0)
+    subst h
+    reduceGoal
+    rw [neg_zero]
   id_closure := rfl
 
 instance kernel_group : Group (Metabelian.Kernel Q K) :=
   subGroup.Group _
 
-instance kernel_inclusion : Group.Homomorphism (subType.val (λ ((k, q) : K × Q) => q = (0 : Q))) := inferInstance
+instance kernel_inclusion : Group.Homomorphism (subType.val (λ ((_, q) : K × Q) => q = (0 : Q))) := inferInstance
 
 theorem Metabelian.Kernel.mul_comm : ∀ k k' : Metabelian.Kernel Q K, k * k' = k' * k := by
   intro ⟨⟨ka, 0⟩, rfl⟩; intro ⟨⟨kb, 0⟩, rfl⟩
   apply subType.eq_of_val_eq
-  show Mul.mul (ka, (0 : Q)) (kb, 0) = Mul.mul (kb, 0) (ka, 0)
-  simp [Mul.mul, MetabelianGroup.mul]; rw [add_comm]
+  show (ka, (0 : Q)) * (kb, 0) = (kb, 0) * (ka, 0)
+  repeat (rw [MetabelianGroup.mult])
+  simp only [add_zero, Cocycle.cocycleId, AddCommGroup.Action.id_action, add_comm]
 
-instance : AddCommGroup (Metabelian.Kernel Q K) := Group.to_additive (Metabelian.Kernel.mul_comm _ _ _)
+instance kernel_addgroup : AddCommGroup (Metabelian.Kernel Q K) :=
+  Group.to_additive (Metabelian.Kernel.mul_comm Q K c)
 
 instance : AddCommGroup.Homomorphism (Metabelian.Kernel.inclusion Q K) where
   add_dist := by
     intro k k'
-    simp [Metabelian.Kernel.inclusion]
+    show _ = ⟨(k, 0) * (k', 0), _⟩
     apply subType.eq_of_val_eq
-    show (k + k', (0 : Q)) = Mul.mul (k, 0) (k', 0)
-    simp [Mul.mul, MetabelianGroup.mul]
+    show ((k + k'), (0 : Q)) = (k, (0 : Q)) * (k', (0 : Q))
+    rw [MetabelianGroup.mult]
+    simp
 
 instance : AddCommGroup.Homomorphism (Metabelian.Kernel.projection Q K) where
   add_dist := by
     intro ⟨⟨k, 0⟩, rfl⟩; intro ⟨⟨k', 0⟩, rfl⟩
-    simp [Metabelian.Kernel.projection, MetabelianGroup.mul]
+    -- show (Metabelian.Kernel.projection Q K) ⟨(k, (0 : Q)) * (k', (0 : Q)), _⟩ = k + k'
+    show (fun (k, _) => k) ((k, (0 : Q)) * (k', (0 : Q))) = k + k'
+    reduceGoal
+    -- show k + (0 : Q) • k' + c 0 0 = k + k'
+    simp
 
 instance : AddCommGroup.Isomorphism K (Metabelian.Kernel Q K) :=
   {
@@ -195,8 +216,16 @@ instance : AddCommGroup.Isomorphism K (Metabelian.Kernel Q K) :=
     mapHom := inferInstance
     inv := Metabelian.Kernel.projection Q K
     invHom := inferInstance
-    idSrc := by apply funext; intro; simp [Metabelian.Kernel.projection, Metabelian.Kernel.inclusion]
-    idTgt := by apply funext; intro ⟨⟨k, 0⟩, rfl⟩; simp [Metabelian.Kernel.projection, Metabelian.Kernel.inclusion]
+    idSrc := by 
+              apply funext
+              intro x
+              show (Metabelian.Kernel.projection Q K) ((Metabelian.Kernel.inclusion Q K) x) = x 
+              rw [Metabelian.Kernel.projection, Metabelian.Kernel.inclusion]
+    idTgt := by 
+              apply funext 
+              intro ⟨⟨k, 0⟩, rfl⟩
+              show (Metabelian.Kernel.inclusion Q K) ((Metabelian.Kernel.projection Q K) ⟨⟨k, 0⟩, rfl⟩) = ⟨⟨k, 0⟩, rfl⟩
+              rw [Metabelian.Kernel.projection, Metabelian.Kernel.inclusion]
   }
 
 end Exactness
