git/Augustindou/natural2lean-lean-project-template/LeanUtils/Tactic.lean
@@ -1,32 +1,9 @@
 import LeanUtils.Div
 import LeanUtils.Parity
 
--- Better simp
 attribute [simp]
-    -- addition
-      -- swapping
-      Nat.add_assoc
-      Nat.add_comm
-      Nat.add_left_comm
-    -- multiplication
-      -- swapping
-      Nat.mul_assoc
-      Nat.mul_comm
-      Nat.mul_left_comm
-      -- zero & one
-      Nat.mul_zero
-      Nat.zero_mul
-      Nat.mul_one
-      Nat.one_mul
-    -- powers
-      -- zero & one
-      Nat.pow_zero
-    -- multiplication to addition
-    Nat.left_distrib
-    Nat.right_distrib
-
-    -- defined in LeanUtils
-    Nat.divisible
-    Nat.mod_rewrite
-    Nat.even
-    Nat.odd
+  -- defined in LeanUtils
+  Nat.divisible
+  Nat.mod_rewrite
+  Nat.even
+  Nat.odd
