git/Augustindou/natural2lean-lean-project-template/examples/in-progress/n-cube/theorem.lean
@@ -3,28 +3,27 @@ open Nat
 
 theorem n_cube_plus_2_n (n : Nat) : divisible 3 (n^3 + 2*n) := by
   match n with
-  | 0 => trivial
+  | 0 => repeat (first | rfl | trivial | ring | simp_all)
   | k+1 => 
     have h₁ : divisible 3 (k ^ 3 + 2 * k) := n_cube_plus_2_n k
-    
-    have ⟨z, h₂⟩ : ∃ z, k^3 + 2*k = 3*z := by simp_all
+
+    have ⟨z, h₂⟩ : ∃ z, k^3 + 2*k = 3*z := by
+      repeat (first | ring | simp_all)
     
     have h₃ : (k + 1) ^ 3 + 2 * (k + 1) = 3*(z + k^2 + k + 1) := by
       calc
         (k + 1) ^ 3 + 2 * (k + 1) = k^3 + 3*k^2 + 5*k + 3 := by 
-          try simp_all
-          try ring
+          repeat (first | ring | simp_all)
         _ = k^3 + 2*k + 3 * (k^2 + k + 1) := by 
-          admit
+          repeat (first | ring | simp_all)
         _ = 3*z + 3 * (k^2 + k + 1) := by
-          try simp_all
-          try ring
+          repeat (first | ring | simp_all)
         _ = 3 * (z + k^2 + k + 1) := by
-          try simp_all
-          try ring
-    
-    rw [divisible]
+          repeat (first | ring | simp_all)
+    try rw [h₃]
+  
+    apply mod_rewrite.mpr
+    exact ⟨_, by repeat (first | rfl | assumption | ring | simp_all)⟩
 
-    exact ⟨_, by admit⟩
-    
+  
 
