git/Augustindou/natural2lean-lean-project-template/examples/working/contrapositive/theorem.lean
@@ -12,24 +12,26 @@ theorem square_mod_3 (q : Nat) : (¬divisible 3 q) → (q^2 % 3 = 1) := by
 
   contradiction
 
-  have ⟨k, h3⟩ : ∃ (k : Nat), q = 3 * k + 1 := by 
-    simp at *
-    assumption
+  have ⟨k, h3⟩ : ∃ (k : Nat), q = 3 * k + 1 := by simp_all
 
   have q_square : q^2 = 3 * (3 * k^2 + 2 * k) + 1  := by 
     calc
-      q^2 = (3 * k + 1)^2 := by try simp [*]; try ring
-      _ = 9 * k^2 + 6 * k + 1 := by try simp [*]; try ring
-      _ = 3 * (3 * k^2 + 2 * k) + 1 := by try simp [*]; try ring
+      q^2 = (3 * k + 1)^2 := by 
+        repeat (first | ring | simp_all)
+      _ = 9 * k^2 + 6 * k + 1 := by 
+        repeat (first | ring | simp_all)
+      _ = 3 * (3 * k^2 + 2 * k) + 1 := by 
+        repeat (first | ring | simp_all)
   exact ⟨_, by assumption⟩
 
-  have ⟨k, h3⟩ : ∃ (k : Nat), q = 3 * k + 2 := by 
-    simp at *
-    assumption
+  have ⟨k, h3⟩ : ∃ (k : Nat), q = 3 * k + 2 := by simp_all
+  
   have q_square : q^2 = 3 * (3 * k^2 + 4 * k + 1) + 1 := by 
     calc
-      q^2 = (3 * k + 2)^2 := by try simp [*]; try ring
-      _ = 3 * (3 * k^2 + 4 * k + 1) + 1 := by try simp [*]; try ring
+      q^2 = (3 * k + 2)^2 := by 
+        repeat (first | ring | simp_all)
+      _ = 3 * (3 * k^2 + 4 * k + 1) + 1 := by 
+        repeat (first | ring | simp_all)
   
   exact ⟨_, by assumption⟩
 
@@ -42,8 +44,7 @@ theorem square_of_q_divisible_by_3_means_q_is_divisible_by_3 (q : Nat) (h₁ : d
   intro h₁
 
   have h₂ : q^2 % 3 = 1 := by
-    try simp_all [square_mod_3]
-    try ring
+    repeat (first | ring | simp_all [square_mod_3])
 
   simp_all
   
