git/Augustindou/natural2lean-lean-project-template/examples/working/sqr_m-even/theorem.lean
@@ -8,14 +8,11 @@ theorem square_of_even_number_is_even (m : Nat) : (even m) → (even (m ^ 2)) :=
   have h₃ : m^2 = 2*(2*n^2) := by 
     calc
       m^2 = (2*n)^2 := by 
-        try simp [*]
-        try ring
+        repeat (first | ring | simp_all)
       _ = 4*n^2 := by 
-        try simp [*]
-        try ring
+        repeat (first | ring | simp_all)
       _ = 2*(2*n^2) := by 
-        try simp [*]
-        try ring
+        repeat (first | ring | simp_all)
   
   exact ⟨_, by assumption⟩
 
