git/Augustindou/natural2lean-lean-project-template/examples/working/sqr_q-mod-3/theorem.lean
@@ -16,18 +16,22 @@ theorem square_mod_3 (q : Nat) : (¬divisible 3 q) → (q^2 % 3 = 1) := by
 
   have q_square : q^2 = 3 * (3 * k^2 + 2 * k) + 1  := by 
     calc
-      q^2 = (3 * k + 1)^2 := by try simp [*]; try ring
-      _ = 9 * k^2 + 6 * k + 1 := by try simp [*]; try ring
-      _ = 3 * (3 * k^2 + 2 * k) + 1 := by try simp [*]; try ring
+      q^2 = (3 * k + 1)^2 := by 
+        repeat (first | ring | simp_all)
+      _ = 9 * k^2 + 6 * k + 1 := by 
+        repeat (first | ring | simp_all)
+      _ = 3 * (3 * k^2 + 2 * k) + 1 := by 
+        repeat (first | ring | simp_all)
   
   exact ⟨_, by assumption⟩
 
   have ⟨k, h3⟩ : ∃ (k : Nat), q = 3 * k + 2 := by 
-    simp at *
-    assumption
+    simp_all
   have q_square : q^2 = 3 * (3 * k^2 + 4 * k + 1) + 1 := by 
     calc
-      q^2 = (3 * k + 2)^2 := by try simp [*]; try ring
-      _ = 3 * (3 * k^2 + 4 * k + 1) + 1 := by try simp [*]; try ring
+      q^2 = (3 * k + 2)^2 := by 
+        repeat (first | ring | simp_all)
+      _ = 3 * (3 * k^2 + 4 * k + 1) + 1 := by 
+        repeat (first | ring | simp_all)
   
   exact ⟨_, by assumption⟩
