git/g4rgoil/tba-project/TBA/While/Solution.lean
@@ -2,6 +2,46 @@ import TBA.While.Semantics
 
 namespace While
 
--- Now it's your turn!
+namespace Optimisation
+
+def foldExpr (σ : State) : Expr → Expr
+  | .const v => Expr.const v
+  | .var x =>
+    match σ x with
+    | some v => Expr.const v
+    | none   => Expr.var x
+  | .binop e₁ op e₂ =>
+    match foldExpr σ e₁, foldExpr σ e₂ with
+    | .const v₁, .const v₂ =>
+      match op.eval v₁ v₂ with
+      | some v => Expr.const v
+      | none   => Expr.binop v₁ op v₂
+    | e₁', e₂' => Expr.binop e₁' op e₂'
+
+def foldCom (σ : State) : Com → (Com × State)
+  | .skip => (Com.skip, σ)
+  | .ass x e => 
+      match foldExpr σ e with
+      | .const v => (Com.ass x v, σ[x ↦ v])
+      | e'       => (Com.ass x e', σ[x ↦ none])
+  | .seq c₁ c₂ =>
+    have (c₁', σ')  := foldCom σ c₁
+    have (c₂', σ'') := foldCom σ' c₂
+    (Com.seq c₁' c₂', σ'')
+  | .cond b cₜ cₑ => 
+    match foldExpr σ b with
+    | .const true  => foldCom σ cₜ
+    | .const false => foldCom σ cₑ
+    | b' =>
+      have ((cₜ', σₜ), (cₑ', σₑ)) := (foldCom σ cₜ, foldCom σ cₑ)
+      (Com.cond b' cₜ' cₑ', λ k => if σₜ k = σₑ k then σₜ k else none)
+  | .while b c =>
+    match foldExpr σ b with
+    | .const false => (Com.skip, σ)
+    | _            => (Com.while b (foldCom Map.empty c).1, Map.empty)
+
+def optimise : Com → Com := λ c => (foldCom Map.empty c).1
+
+end Optimisation
 
 end While
