git/g4rgoil/tba-project/TBA/While/Testing.lean
@@ -1,0 +1,65 @@
+import TBA.While.Solution
+
+namespace While
+
+namespace Optimisation
+
+#reduce foldExpr Map.empty `[Expr| 5 + 4 - 9 = 0]
+#reduce foldExpr Map.empty `[Expr| 1 - 4 < (5 + 5) - (10 + 3)]
+#reduce foldExpr Map.empty `[Expr| 1 + true]
+
+def com1 := `[Com| 
+  x := 7;
+  y := 3;
+  if (x = y) {
+    y := x + 2;
+  } else {
+    y := x - z;
+    z := y;
+  }]
+#reduce optimise com1
+
+def com2 := `[Com| 
+  x := 2;
+  y := x;
+  b := x = y;
+  if (b) {
+    z := x + y;
+  } else {
+    z := x;
+  }]
+#reduce optimise com2
+
+def com3 := `[Com|
+  x := 13;
+  y := 7;
+  while (y = x - 5) {
+    x := x + 1;
+  }]
+#reduce optimise com3
+
+def com4 := `[Com|
+  x := 8;
+  if (x < y) {
+    x := x + 1;
+  } else {
+    y := y + 3;
+    x := 9;
+  }
+  y := x;]
+#reduce optimise com4
+
+def com5 := `[Com|
+  if (x < y) {
+    x := 9;
+    y := x + 1;
+  } else {
+    x := 9;
+    y := x - 1;
+  }
+  z := x + y;]
+#reduce optimise com5
+
+end Optimisation
+
+end While
