git/larsk21/iris-lean/src/Iris/Proofmode/Tactics.lean
@@ -1,20 +1,21 @@
 import Iris.BI
 import Iris.Proofmode.Environments
 import Iris.Proofmode.Expr
+import Iris.Proofmode.InputPatterns
 import Iris.Proofmode.Theorems
 import Iris.Std
 
 import Lean.Elab
 
 namespace Iris.Proofmode
-open Iris.BI
+open Iris.BI Iris.Std
 open Lean Lean.Elab Lean.Elab.Tactic Lean.Meta
 
 namespace Internal
 end Internal
 open Internal
 
-elab "iStartProof" : tactic => do
+elab "istart_proof" : tactic => do
   -- parse goal
   let goal :: _ ← getUnsolvedGoals
     | throwNoGoalsToBeSolved
@@ -31,7 +32,7 @@ elab "iStartProof" : tactic => do
   ))
   catch _ => throwError "unable to start proof mode"
 
-elab "iStopProof" : tactic => do
+elab "istop_proof" : tactic => do
   -- parse goal
   let goal :: _ ← getUnsolvedGoals
     | throwNoGoalsToBeSolved
@@ -49,10 +50,10 @@ elab "iStopProof" : tactic => do
   catch _ => throwError "unable to stop proof mode"
 
 
-private def extractEnvsEntailsFromGoal? (startProofMode : Bool := false) : TacticM <| Expr × Expr × Expr := do
+private def extractEnvsEntailsFromGoal (startProofMode : Bool := false) : TacticM <| Expr × Expr × Expr := do
   if startProofMode then
     evalTactic (← `(tactic|
-      iStartProof
+      istart_proof
     ))
 
   let goal :: _ ← getUnsolvedGoals
@@ -64,29 +65,21 @@ private def extractEnvsEntailsFromGoal? (startProofMode : Bool := false) : Tacti
 
   return envsEntails
 
-private def findHypothesis? (name : Name) (Γₚ Γₛ : Expr) : TacticM <| HypothesisType × Nat := do
+private def findHypothesis (name : Name) : TacticM HypothesisIndex := do
+  let (Γₚ, Γₛ, _) ← extractEnvsEntailsFromGoal
   if let some i ← Γₚ.asListExpr_findIndex? (·.getMDataName?.isEqSome name) then
-    return (.intuitionistic, i)
+    let some l ← Γₚ.asListExpr_length?
+      | throwError "ill-formed proof environment"
+    return ⟨.intuitionistic, i, l⟩
   else if let some i ← Γₛ.asListExpr_findIndex? (·.getMDataName?.isEqSome name) then
-    return (.spatial, i)
+    let some l ← Γₛ.asListExpr_length?
+      | throwError "ill-formed proof environment"
+    return ⟨.spatial, i, l⟩
   else
     throwError "unknown hypothesis"
 
 
-namespace Internal
-
-scoped elab "iRename " categ:(&"p" <|> &"s") idx:num colGt name:ident : tactic => do
-  -- parse syntax
-  let categ ← match categ.getKind with
-    | `p => pure HypothesisType.intuitionistic
-    | `s => pure HypothesisType.spatial
-    | _  => throwUnsupportedSyntax
-  let some idx := idx.isNatLit?
-    | throwUnsupportedSyntax
-  let name := name.getId
-  if name.isAnonymous then
-    throwUnsupportedSyntax
-
+def Internal.irenameCore (hypIndex : HypothesisIndex) (name : Name) : TacticM Unit := do
   -- parse goal
   let goal :: _ ← getUnsolvedGoals
     | throwNoGoalsToBeSolved
@@ -95,25 +88,32 @@ scoped elab "iRename " categ:(&"p" <|> &"s") idx:num colGt name:ident : tactic =
   let some (Γₚ, Γₛ, _) := extractEnvsEntails? expr
     | throwError "not in proof mode"
 
-  -- check for unique hypothesis name
-  if ← [Γₚ, Γₛ].anyM (fun Γ => do return (← Γ.asListExpr_any? (·.getMDataName?.isEqSome name)) matches some true) then
-    throwError "name is already used for another hypothesis"
+  let modifyHypothesis (Γ : Expr) (idx : Nat) : TacticM Expr := do
+    -- find hypothesis
+    let some h ← Γ.asListExpr_get? idx
+      | throwError "invalid index or ill-formed proof environment"
 
-  -- find hypothesis
-  let Γ := match categ with
-    | .intuitionistic => Γₚ
-    | .spatial        => Γₛ
-  let some h ← Γ.asListExpr_get? idx
-    | throwError "invalid index or ill-formed proof environment"
+    -- check for unique (or equal) hypothesis name
+    let nameFrom? := h.getMDataName?
+    if nameFrom? |>.map (· != name) |>.getD true then
+      if ← [Γₚ, Γₛ].anyM (fun Γ => do return (← Γ.asListExpr_any? (·.getMDataName?.isEqSome name)) matches some true) then
+        throwError "name is already used for another hypothesis"
 
-  -- rename
-  let h := h.setMDataName? name
+    -- rename hypothesis
+    let h := h.setMDataName? name
 
-  -- insert modified hypothesis
-  let some Γ ← Γ.asListExpr_set? h idx
-    | throwError "invalid index or ill-formed proof environment"
-  let Γₚ := if categ matches .intuitionistic then Γ else Γₚ
-  let Γₛ := if categ matches .spatial        then Γ else Γₛ
+    -- re-insert hypothesis
+    let some Γ ← Γ.asListExpr_set? h idx
+      | throwError "invalid index or ill-formed proof environment"
+
+    return Γ
+
+  -- modify environment
+  let (Γₚ, Γₛ) ← match hypIndex with
+    | ⟨.intuitionistic, index, _⟩ => do
+      pure (← modifyHypothesis Γₚ index, Γₛ)
+    | ⟨.spatial, index, _⟩ => do
+      pure (Γₚ, ← modifyHypothesis Γₛ index)
 
   -- update goal
   let some expr := modifyEnvsEntails? expr Γₚ Γₛ none
@@ -121,129 +121,109 @@ scoped elab "iRename " categ:(&"p" <|> &"s") idx:num colGt name:ident : tactic =
 
   setMVarType goal expr
 
-end Internal
-
-elab "iRename " colGt nameFrom:ident " into " colGt nameTo:ident : tactic => do
+elab "irename" colGt nameFrom:ident "into" colGt nameTo:ident : tactic => do
   -- parse syntax
   if nameFrom.getId.isAnonymous then
     throwUnsupportedSyntax
-  if nameTo.getId.isAnonymous then
+  let nameTo := nameTo.getId
+  if nameTo.isAnonymous then
     throwUnsupportedSyntax
 
-  -- extract environment
-  let (Γₚ, Γₛ, _) ← extractEnvsEntailsFromGoal? true
-
-  -- find hypothesis index and rename hypothesis
-  match ← findHypothesis? nameFrom.getId Γₚ Γₛ with
-    | (.intuitionistic, i) => evalTactic (← `(tactic| iRename p $(quote i) $nameTo))
-    | (.spatial, i)        => evalTactic (← `(tactic| iRename s $(quote i) $nameTo))
+  -- find and rename hypothesis
+  irenameCore (← findHypothesis nameFrom.getId) nameTo
 
 
-elab "iClear" colGt name:ident : tactic => do
+elab "iclear" colGt name:ident : tactic => do
   -- parse syntax
   let name := name.getId
   if name.isAnonymous then
     throwUnsupportedSyntax
 
-  -- extract environment
-  let (Γₚ, Γₛ, _) ← extractEnvsEntailsFromGoal? true
-
-  let (some lₚ, some lₛ) ← (Γₚ, Γₛ).mapAllM (M := MetaM) Lean.Expr.asListExpr_length?
-    | throwError "ill-formed proof environment"
-
   -- find hypothesis index
-  let envsIndex ← match ← findHypothesis? name Γₚ Γₛ with
-    | (.intuitionistic, i) => `(EnvsIndex.p ⟨$(quote i), by show $(quote i) < $(quote lₚ) ; decide⟩)
-    | (.spatial,        i) => `(EnvsIndex.s ⟨$(quote i), by show $(quote i) < $(quote lₛ) ; decide⟩)
+  let hypIndex ← findHypothesis name
 
   -- clear hypothesis
   try evalTactic (← `(tactic|
     first
-    | refine tac_clear $envsIndex _ ?_
+    | refine tac_clear $(← hypIndex.quoteAsEnvsIndex) _ ?_
     | fail
   ))
   catch _ => throwError "failed to clear the hypothesis"
 
 
-elab "iIntro " colGt name:ident : tactic => do
-  -- parse syntax
-  if name.getId.isAnonymous then
-    throwUnsupportedSyntax
-
+def Internal.iintroCore (type : HypothesisType) (name : Name) : TacticM Unit := do
   -- extract environment
-  let (_, Γₛ, _) ← extractEnvsEntailsFromGoal? true
+  let (Γₚ, Γₛ, _) ← extractEnvsEntailsFromGoal true
 
   -- determine hypothesis list length
-  let some s_length ← Γₛ.asListExpr_length?
+  let (some lₚ, some lₛ) ← (Γₚ, Γₛ).mapAllM (·.asListExpr_length?)
     | throwError "ill-formed proof environment"
 
-  -- introduce hypothesis
+  match type with
+  | .intuitionistic =>
+    -- introduce hypothesis
+    try evalTactic (← `(tactic|
+      first
+      | refine tac_impl_intro_intuitionistic _ ?_
+      | refine tac_wand_intro_intuitionistic _ ?_
+      | fail
+    ))
+    catch _ => throwError "failed to introduce hypothesis"
+
+    -- name hypothesis
+    irenameCore ⟨.intuitionistic, lₚ, lₚ + 1⟩ name
+  | .spatial =>
+    -- introduce hypothesis
+    try evalTactic (← `(tactic|
+      first
+      | refine tac_impl_intro _ ?_
+      | refine tac_wand_intro _ ?_
+      | fail
+    ))
+    catch _ => throwError "failed to introduce hypothesis"
+
+    -- name hypothesis
+    irenameCore ⟨.spatial, lₛ, lₛ + 1⟩ name
+
+def Internal.iintroCoreClear : TacticM Unit := do
+  -- drop implication premise
   try evalTactic (← `(tactic|
     first
-    | refine tac_impl_intro _ ?_
-    | refine tac_wand_intro _ ?_
+    | istart_proof
+      refine tac_impl_intro_drop _ ?_
     | fail
-  ))
-  catch _ => throwError "failed to introduce hypothesis"
+  )) catch _ => throwError "failed to drop implication hypothesis"
 
-  -- name hypothesis
-  evalTactic (← `(tactic|
-    iRename s $(quote s_length) $name
-  ))
-
-elab "iIntro " colGt "#" colGt name:ident : tactic => do
-  -- parse syntax
-  if name.getId.isAnonymous then
-    throwUnsupportedSyntax
-
-  -- extract environment
-  let (Γₚ, _, _) ← extractEnvsEntailsFromGoal? true
-
-  -- determine hypothesis list length
-  let some p_length ← Γₚ.asListExpr_length?
-    | throwError "ill-formed proof environment"
-
-  -- introduce hypothesis
+def Internal.iintroCoreForall (name : Name) : TacticM Unit := do
+  -- introduce universally bound variable
   try evalTactic (← `(tactic|
     first
-    | refine tac_impl_intro_intuitionistic _ ?_
-    | refine tac_wand_intro_intuitionistic _ ?_
+    | istart_proof
+      refine tac_forall_intro _ ?_
+      intro $(mkIdent name)
     | fail
   ))
-  catch _ => throwError "failed to introduce hypothesis"
-
-  -- name hypothesis
-  evalTactic (← `(tactic|
-    iRename p $(quote p_length) $name
-  ))
+  catch _ => throwError "failed to introduce universally bound variable"
 
 
-elab "iExact " colGt name:ident : tactic => do
+elab "iexact" colGt name:ident : tactic => do
   -- parse syntax
   let name := name.getId
   if name.isAnonymous then
     throwUnsupportedSyntax
 
-  -- extract environment
-  let (Γₚ, Γₛ, _) ← extractEnvsEntailsFromGoal?
-
-  let (some lₚ, some lₛ) ← (Γₚ, Γₛ).mapAllM (M := MetaM) Lean.Expr.asListExpr_length?
-    | throwError "ill-formed proof environment"
-
   -- find hypothesis index
-  let envsIndex ← match ← findHypothesis? name Γₚ Γₛ with
-    | (.intuitionistic, i) => `(EnvsIndex.p ⟨$(quote i), by show $(quote i) < $(quote lₚ) ; decide⟩)
-    | (.spatial,        i) => `(EnvsIndex.s ⟨$(quote i), by show $(quote i) < $(quote lₛ) ; decide⟩)
+  let hypIndex ← findHypothesis name
 
   -- try to solve the goal with the found hypothesis
   try evalTactic (← `(tactic|
     first
-    | refine tac_assumption $envsIndex _
+    | refine tac_assumption $(← hypIndex.quoteAsEnvsIndex) _
     | fail
   ))
   catch _ => throwError "failed to use the hypothesis to close the goal"
 
-elab "iAssumptionLean" : tactic => do
+elab "iassumption_lean" : tactic => do
   -- try all hypotheses from the local context
   let hs ← getLCtx
   for h in ← getLCtx do
@@ -263,9 +243,9 @@ elab "iAssumptionLean" : tactic => do
 
   throwError "no matching hypothesis found or remaining environment cannot be cleared"
 
-elab "iAssumption" : tactic => do
+elab "iassumption" : tactic => do
   -- extract environment
-  let (Γₚ, Γₛ, _) ← extractEnvsEntailsFromGoal?
+  let (Γₚ, Γₛ, _) ← extractEnvsEntailsFromGoal
 
   let (some lₚ, some lₛ) ← (Γₚ, Γₛ).mapAllM (M := MetaM) Lean.Expr.asListExpr_length?
     | throwError "ill-formed proof environment"
@@ -284,28 +264,93 @@ elab "iAssumption" : tactic => do
 
   -- try all available hypotheses
   for i in List.range lₚ do
-    let envsIndex ← `(EnvsIndex.p ⟨$(quote i), by show $(quote i) < $(quote lₚ) ; decide⟩)
-    if ← tryCloseGoal envsIndex then
+    let hypIndex : HypothesisIndex := ⟨.intuitionistic, i, lₚ⟩
+    if ← tryCloseGoal (← hypIndex.quoteAsEnvsIndex) then
       return ()
 
   for i in List.range lₛ do
-    let envsIndex ← `(EnvsIndex.s ⟨$(quote i), by show $(quote i) < $(quote lₛ) ; decide⟩)
-    if ← tryCloseGoal envsIndex then
+    let hypIndex : HypothesisIndex := ⟨.spatial, i, lₛ⟩
+    if ← tryCloseGoal (← hypIndex.quoteAsEnvsIndex) then
       return ()
 
   -- try all hypotheses from the Lean context
   try evalTactic (← `(tactic|
     first
-    | iAssumptionLean
+    | iassumption_lean
     | fail
   ))
   catch _ => throwError "no matching hypothesis found or remaining environment cannot be cleared"
 
 
-elab "iSplit" : tactic => do
+elab "ipure" name:ident : tactic => do
+  -- parse syntax
+  if name.getId.isAnonymous then
+    throwUnsupportedSyntax
+
+  -- find hypothesis index
+  let hypIndex ← findHypothesis name.getId
+
+  -- move hypothesis
+  try evalTactic (← `(tactic|
+    first
+    | refine tac_pure $(← hypIndex.quoteAsEnvsIndex) _ ?_
+      intro $name
+    | fail
+  )) catch _ => throwError "could not move hypothesis to the Lean context"
+
+elab "iintuitionistic" name:ident : tactic => do
+  -- parse syntax
+  let name := name.getId
+  if name.isAnonymous then
+    throwUnsupportedSyntax
+
+  -- find hypothesis index
+  let hypIndex ← findHypothesis name
+
+  -- move hypothesis
+  try evalTactic (← `(tactic|
+    first
+    | refine tac_intuitionistic $(← hypIndex.quoteAsEnvsIndex) _ ?_
+    | fail
+  )) catch _ => throwError "could not move hypothesis to the intuitionistic context"
+
+  -- extract environment
+  let (Γₚ, _, _) ← extractEnvsEntailsFromGoal
+  let some lₚ ← Γₚ.asListExpr_length?
+    | throwError "ill-formed proof environment"
+
+  -- re-name hypothesis
+  irenameCore ⟨.intuitionistic, lₚ - 1, lₚ⟩ name
+
+elab "ispatial" name:ident : tactic => do
+  -- parse syntax
+  let name := name.getId
+  if name.isAnonymous then
+    throwUnsupportedSyntax
+
+  -- find hypothesis index
+  let hypIndex ← findHypothesis name
+
+  -- move hypothesis
+  try evalTactic (← `(tactic|
+    first
+    | refine tac_spatial $(← hypIndex.quoteAsEnvsIndex) _ ?_
+    | fail
+  )) catch _ => throwError "could not move hypothesis to the spatial context"
+
+  -- extract environment
+  let (_, Γₛ, _) ← extractEnvsEntailsFromGoal
+  let some lₛ ← Γₛ.asListExpr_length?
+    | throwError "ill-formed proof environment"
+
+  -- re-name hypothesis
+  irenameCore ⟨.spatial, lₛ - 1, lₛ⟩ name
+
+
+elab "isplit" : tactic => do
   -- start proof mode if not already
   evalTactic (← `(tactic|
-    iStartProof
+    istart_proof
   ))
 
   -- split conjunction
@@ -316,13 +361,11 @@ elab "iSplit" : tactic => do
   ))
   catch _ => throwError "unable to split conjunction"
 
-namespace Internal
-
-scoped elab "iSplit" side:(&"L" <|> &"R") "[" names:sepBy(ident, ",") "]" : tactic => do
+elab "isplit" side:(&"l" <|> &"r") "[" names:ident,* "]" : tactic => do
   -- parse syntax
   let splitRight ← match side.getKind with
-    | `L => pure false
-    | `R => pure true
+    | `l => pure false
+    | `r => pure true
     | _  => throwUnsupportedSyntax
   let names ← names.getElems.mapM (fun name => do
     let name := name.getId
@@ -332,7 +375,7 @@ scoped elab "iSplit" side:(&"L" <|> &"R") "[" names:sepBy(ident, ",") "]" : tact
   )
 
   -- extract environment
-  let (_, Γₛ, _) ← extractEnvsEntailsFromGoal? true
+  let (_, Γₛ, _) ← extractEnvsEntailsFromGoal true
 
   -- find indices
   let indices ← names.mapM (fun name => do
@@ -350,12 +393,269 @@ scoped elab "iSplit" side:(&"L" <|> &"R") "[" names:sepBy(ident, ",") "]" : tact
   ))
   catch _ => throwError "unable to split separating conjunction"
 
-end Internal
+macro "isplit" &"l" : tactic => `(tactic| isplit r [])
+macro "isplit" &"r" : tactic => `(tactic| isplit l [])
 
-macro "iSplitL" "[" names:sepBy(ident, ",") "]" : tactic => `(tactic| iSplit L [$[$names:ident],*])
-macro "iSplitR" "[" names:sepBy(ident, ",") "]" : tactic => `(tactic| iSplit R [$[$names:ident],*])
 
-macro "iSplitL" : tactic => `(tactic| iSplit R [])
-macro "iSplitR" : tactic => `(tactic| iSplit L [])
+mutual
+  private partial def Internal.icasesCoreConjunction (hypIndex : HypothesisIndex) (args : Array iCasesPat) : TacticM Unit := do
+    if args.size < 2 then
+      throwError "conjunction must contain at least two elements"
+
+    -- destruct hypothesis with multiple conjunctions
+    let mut remainingArguments := #[(.anonymous, args[0])]
+    let mut hypIndex := hypIndex
+    for i in [:args.size - 1] do
+      -- destruct hypothesis and clear one side if requested
+      let (h, ra) ← (do
+        if args[i] matches .clear then
+          if let some result ← destructRight hypIndex args[i] args[i + 1] then
+            return result
+        else if i + 1 == args.size - 1 && args[i + 1] matches .clear then
+          if let some result ← destructLeft hypIndex args[i] args[i + 1] then
+            return result
+
+        let some result ← destruct hypIndex args[i] args[i + 1]
+          | throwError "failed to destruct conjunction"
+        return result)
+
+      -- update hypothesis index and collect remaining arguments
+      hypIndex := h
+      remainingArguments := remainingArguments |>.pop |>.append ra
+
+    -- process pattern recursively
+    for (name, arg) in remainingArguments do
+      -- save introduced goals
+      let mut goals := []
+
+      -- apply recursive function to each goal
+      for goal in ← getUnsolvedGoals do
+        setGoals [goal]
+        icasesCore name arg
+        goals := goals ++ (← getUnsolvedGoals)
+
+      -- restore all introduced goals
+      setGoals goals
+  where
+    destructRight (hypIndex : HypothesisIndex) (argL argR : iCasesPat) : TacticM <| Option <| HypothesisIndex × (Array <| Name × iCasesPat) := do
+      -- destruct hypothesis
+      try evalTactic (← `(tactic|
+        first
+        | refine tac_conjunction_destruct_choice $(← hypIndex.quoteAsEnvsIndex) false _ ?_
+          simp only [List.concat, ite_true, ite_false]
+        | fail
+      )) catch _ => return none
+
+      -- update hypothesis index
+      let hypIndex := { hypIndex with index := hypIndex.length - 1 }
+
+      -- temporarily name hypothesis
+      let name ← mkFreshUserName `i
+      irenameCore hypIndex name
+
+      -- return new hypothesis index and remaining arguments
+      return (hypIndex, #[(name, argR)])
+
+    destructLeft (hypIndex : HypothesisIndex) (argL argR : iCasesPat) : TacticM <| Option <| HypothesisIndex × (Array <| Name × iCasesPat) := do
+      -- destruct hypothesis
+      try evalTactic (← `(tactic|
+        first
+        | refine tac_conjunction_destruct_choice $(← hypIndex.quoteAsEnvsIndex) true _ ?_
+          simp only [List.concat, ite_true, ite_false]
+        | fail
+      )) catch _ => return none
+
+      -- update hypothesis index
+      let hypIndex := { hypIndex with index := hypIndex.length - 1 }
+
+      -- temporarily name hypothesis
+      let name ← mkFreshUserName `i
+      irenameCore hypIndex name
+
+      -- return new hypothesis index and remaining arguments
+      return (hypIndex, #[(name, argL)])
+
+    destruct (hypIndex : HypothesisIndex) (argL argR : iCasesPat) : TacticM <| Option <| HypothesisIndex × (Array <| Name × iCasesPat) := do
+      -- destruct hypothesis
+      try evalTactic (← `(tactic|
+        first
+        | refine tac_conjunction_destruct $(← hypIndex.quoteAsEnvsIndex) _ ?_
+          simp only [List.concat]
+        | fail
+      ))
+      catch _ => return none
+
+      -- update hypothesis index
+      let hypIndex := { hypIndex with index := hypIndex.length, length := hypIndex.length + 1 }
+
+      -- temporarily name hypotheses
+      let nameL ← mkFreshUserName `i
+      let nameR ← mkFreshUserName `i
+
+      irenameCore { hypIndex with index := hypIndex.length - 2 } nameL
+      irenameCore { hypIndex with index := hypIndex.length - 1 } nameR
+
+      -- return new hypothesis index and remaining arguments
+      return (hypIndex, #[(nameL, argL), (nameR, argR)])
+
+  private partial def Internal.icasesCoreDisjunction (hypIndex : HypothesisIndex) (args : Array iCasesPat) (mainGoal : MVarId) : TacticM Unit := do
+    -- find main goal tag
+    let tag ← getMVarTag mainGoal
+
+    let mut goalsInd := #[mainGoal]
+    let mut hypIndex := hypIndex
+    for i in [1:args.size] do
+      -- assemble new goal tags
+      let tagL := tag ++ s!"Ind_{i}".toName
+      let tagR := if i < args.size - 1 then
+        tag ++ s!"Ind_{i + 1}_tmp".toName
+      else
+        tag ++ s!"Ind_{i + 1}".toName
+
+      -- destruct hypothesis
+      try evalTactic (← `(tactic|
+        first
+        | refine tac_disjunction_destruct $(← hypIndex.quoteAsEnvsIndex) _
+            ?$(mkIdent <| tagL):ident
+            ?$(mkIdent <| tagR):ident
+          <;> simp only [List.concat]
+        | fail
+      ))
+      catch _ => throwError "failed to destruct disjunction"
+
+      -- update hypothesis index for new goals
+      hypIndex := { hypIndex with index := hypIndex.length - 1 }
+
+      -- save new goals
+      let (some goalL, some goalR) ← (tagL, tagR).mapAllM findGoalFromTag?
+        | throwError "goal tag assignment failed"
+      goalsInd := goalsInd |>.pop |>.push goalL |>.push goalR
+
+      -- switch to right new goal
+      setGoals [goalR]
+
+    -- restore all new goals
+    setGoals goalsInd.toList
+
+    -- save goals introduced by recursive calls
+    let mut goalsRec := []
+
+    -- process pattern recursively
+    for (arg, goal) in args.zip goalsInd do
+      let name ← mkFreshUserName `i
+
+      setGoals [goal]
+      irenameCore { hypIndex with index := hypIndex.length - 1 } name
+      icasesCore name arg
+      goalsRec := goalsRec ++ (← getUnsolvedGoals)
+
+    -- restore all introduced goals
+    setGoals goalsRec
+
+  partial def Internal.icasesCore (nameFrom : Name) (pat : iCasesPat) : TacticM Unit := do
+    -- focus on main goal and save state
+    let mainGoal :: remainingGoals ← getUnsolvedGoals
+      | pure ()
+    setGoals [mainGoal]
+
+    -- find hypothesis index
+    let hypIndex ← findHypothesis nameFrom
+
+    -- process pattern
+    match pat with
+    | .one nameTo =>
+      irenameCore hypIndex nameTo
+
+    | .clear =>
+      evalTactic (← `(tactic|
+        iclear $(mkIdent nameFrom)
+      ))
+
+    | .conjunction args =>
+      if let #[] := args then
+        throwError "empty constructor is not a valid icases pattern"
+      else if let #[arg] := args then
+        return ← icasesCore nameFrom arg
+
+      icasesCoreConjunction hypIndex args
+
+    | .disjunction args =>
+      if let #[] := args then
+        throwError "empty list of alternatives is not a valid icases pattern"
+      else if let #[arg] := args then
+        return ← icasesCore nameFrom arg
+
+      icasesCoreDisjunction hypIndex args mainGoal
+
+    | .pure (.one nameTo) =>
+      irenameCore hypIndex nameTo
+
+      evalTactic (← `(tactic|
+        ipure $(mkIdent nameTo)
+      ))
+
+    | .pure _ =>
+      throwError "cannot further destruct a hypothesis after moving it to the Lean context"
+
+    | .intuitionistic pat =>
+      evalTactic (← `(tactic|
+        iintuitionistic $(mkIdent nameFrom)
+      ))
+
+      icasesCore nameFrom pat
+
+    | .spatial pat =>
+      evalTactic (← `(tactic|
+        ispatial $(mkIdent nameFrom)
+      ))
+
+      icasesCore nameFrom pat
+
+    -- restore goal state
+    setGoals <| (← getUnsolvedGoals) ++ remainingGoals
+end
+
+elab "icases" colGt name:ident "with" colGt pat:icasesPat : tactic => do
+  -- parse syntax
+  let name := name.getId
+  if name.isAnonymous then
+    throwUnsupportedSyntax
+  let some pat := iCasesPat.parse pat
+    | throwUnsupportedSyntax
+
+  -- process pattern
+  icasesCore name pat
+
+
+elab "iintro" pats:(colGt icasesPat)* : tactic => do
+  -- parse syntax
+  let some pats := pats
+    |>.map iCasesPat.parse
+    |>.sequenceMap id
+    | throwUnsupportedSyntax
+
+  for pat in pats do
+    let tmpName ← mkFreshUserName `i
+
+    -- introduce hypothesis and determine remaining pattern
+    let mut pat? := some pat
+    if pat matches .clear then
+      iintroCoreClear
+      pat? := none
+    else if let .pure (.one name) := pat then
+      try
+        iintroCoreForall name
+        pat? := none
+      catch _ =>
+        iintroCore .spatial tmpName
+    else if pat matches .intuitionistic pat then
+      iintroCore .intuitionistic tmpName
+      pat? := some pat
+    else
+      iintroCore .spatial tmpName
+
+    -- process pattern
+    if let some pat := pat? then
+      icasesCore tmpName pat
 
 end Iris.Proofmode
