git/larsk21/iris-lean/src/Iris/Proofmode/Theorems.lean
@@ -38,6 +38,12 @@ theorem tac_impl_intro_intuitionistic [BI PROP] {Γₚ Γₛ : List PROP} {P P' 
   envs_entails ⟨Γₚ, Γₛ⟩ R
 := sorry
 
+theorem tac_impl_intro_drop [BI PROP] {Δ : Envs PROP} {P Q : PROP} (R : PROP) :
+  [FromImpl R P Q] →
+  envs_entails Δ Q →
+  envs_entails Δ R
+:= sorry
+
 theorem tac_wand_intro [BI PROP] {Γₚ Γₛ : List PROP} {P Q : PROP} (R : PROP) :
   [FromWand R P Q] →
   envs_entails ⟨Γₚ, Γₛ.concat P⟩ Q →
@@ -50,6 +56,12 @@ theorem tac_wand_intro_intuitionistic [BI PROP] {Γₚ Γₛ : List PROP} {P P' 
   [TCOr (Affine P) (Absorbing Q)] →
   envs_entails ⟨Γₚ.concat P', Γₛ⟩ Q →
   envs_entails ⟨Γₚ, Γₛ⟩ R
+:= sorry
+
+theorem tac_forall_intro [BI PROP] {Δ : Envs PROP} {Ψ : α → PROP} (Q : PROP) :
+  [FromForall Q Ψ] →
+  (∀ a, envs_entails Δ `[iprop| Ψ a]) →
+  envs_entails Δ Q
 := sorry
 
 -- assumptions
@@ -79,6 +91,45 @@ theorem tac_false_destruct [BI PROP] {Γₚ Γₛ : List PROP} (i : EnvsIndex Γ
   envs_entails ⟨Γₚ, Γₛ⟩ Q
 := sorry
 
+-- moving between contexts
+theorem tac_pure [BI PROP] {Γₚ Γₛ : List PROP} {φ : Prop} (i : EnvsIndex Γₚ.length Γₛ.length) (Q : PROP) :
+   let (p, P) := match i with
+    | .p i => (true, Γₚ.getR i)
+    | .s i => (false, Γₛ.getR i)
+  [IntoPure P φ] →
+  [TCIte p TCTrue (TCOr (Affine P) (Absorbing Q))] →
+   let (Γₚ', Γₛ') := match i with
+    | .p i => (Γₚ.eraseIdxR i, Γₛ)
+    | .s i => (Γₚ, Γₛ.eraseIdxR i)
+  (φ → envs_entails ⟨Γₚ', Γₛ'⟩ Q) →
+  envs_entails ⟨Γₚ, Γₛ⟩ Q
+:= sorry
+
+theorem tac_intuitionistic [BI PROP] {Γₚ Γₛ : List PROP} {P' : PROP} (i : EnvsIndex Γₚ.length Γₛ.length) (Q : PROP) :
+  let (p, P) := match i with
+    | .p i => (true, Γₚ.getR i)
+    | .s i => (false, Γₛ.getR i)
+  [IntoPersistent p P P'] →
+  [TCIte p TCTrue (TCOr (Affine P) (Absorbing Q))] →
+  let (Γₚ', Γₛ') := match i with
+    | .p i => (Γₚ |>.eraseIdxR i |>.concat P', Γₛ)
+    | .s i => (Γₚ.concat P', Γₛ.eraseIdxR i)
+  envs_entails ⟨Γₚ', Γₛ'⟩ Q →
+  envs_entails ⟨Γₚ, Γₛ⟩ Q
+:= sorry
+
+theorem tac_spatial [BI PROP] {Γₚ Γₛ : List PROP} {P' : PROP} (i : EnvsIndex Γₚ.length Γₛ.length) (Q : PROP) :
+  let (p, P) := match i with
+    | .p i => (true, Γₚ.getR i)
+    | .s i => (false, Γₛ.getR i)
+  [FromAffinely P' P p] →
+  let (Γₚ', Γₛ') := match i with
+    | .p i => (Γₚ.eraseIdxR i, Γₛ.concat P')
+    | .s i => (Γₚ, Γₛ |>.eraseIdxR i |>.concat P')
+  envs_entails ⟨Γₚ', Γₛ'⟩ Q →
+  envs_entails ⟨Γₚ, Γₛ⟩ Q
+:= sorry
+
 -- (separating) conjunction splitting
 theorem tac_and_split [BI PROP] {Δ : Envs PROP} {Q1 Q2 : PROP} (P : PROP) :
   [FromAnd P Q1 Q2] →
@@ -94,6 +145,56 @@ theorem tac_sep_split [BI PROP] {Γₚ Γₛ : List PROP} {Q1 Q2 : PROP} (sorted
   envs_entails ⟨Γₚ, Γₛ₁⟩ Q1 →
   envs_entails ⟨Γₚ, Γₛ₂⟩ Q2 →
   envs_entails ⟨Γₚ, Γₛ⟩ P
+:= sorry
+
+-- destruction
+class inductive IntoConjunction [BI PROP] (P : PROP) (P1 P2 : outParam PROP) : Bool → Type
+  | and : [IntoAnd true P P1 P2] → IntoConjunction P P1 P2 true
+  | sep : [IntoSep P P1 P2] → IntoConjunction P P1 P2 false
+
+attribute [instance] IntoConjunction.and
+attribute [instance] IntoConjunction.sep
+
+theorem tac_conjunction_destruct [BI PROP] {Γₚ Γₛ : List PROP} {P1 P2 : PROP} (i : EnvsIndex Γₚ.length Γₛ.length) (Q : PROP) :
+  let (p, P) := match i with
+    | .p i => (true, Γₚ.getR i)
+    | .s i => (false, Γₛ.getR i)
+  [IntoConjunction P P1 P2 p] →
+  let (Γₚ', Γₛ') := match i with
+    | .p i => (Γₚ |>.eraseIdxR i |>.concat P1 |>.concat P2, Γₛ)
+    | .s i => (Γₚ, Γₛ |>.eraseIdxR i |>.concat P1 |>.concat P2)
+  envs_entails ⟨Γₚ', Γₛ'⟩ Q →
+  envs_entails ⟨Γₚ, Γₛ⟩ Q
+:= sorry
+
+theorem tac_conjunction_destruct_choice [BI PROP] {Γₚ Γₛ : List PROP} {P1 P2 : PROP} (i : EnvsIndex Γₚ.length Γₛ.length) (d : Bool) (Q : PROP) :
+  let (p, P) := match i with
+    | .p i => (true, Γₚ.getR i)
+    | .s i => (false, Γₛ.getR i)
+  [IntoAnd p P P1 P2] →
+  let P' := if d then P1 else P2
+  let (Γₚ', Γₛ') := match i with
+    | .p i => (Γₚ |>.eraseIdxR i |>.concat P', Γₛ)
+    | .s i => (Γₚ, Γₛ |>.eraseIdxR i |>.concat P')
+  envs_entails ⟨Γₚ', Γₛ'⟩ Q →
+  envs_entails ⟨Γₚ, Γₛ⟩ Q
+:= sorry
+
+theorem tac_disjunction_destruct [BI PROP] {Γₚ Γₛ : List PROP} {P1 P2 : PROP} (i : EnvsIndex Γₚ.length Γₛ.length) (Q : PROP) :
+  let P := match i with
+    | .p i => Γₚ.getR i
+    | .s i => Γₛ.getR i
+  [IntoOr P P1 P2] →
+  let (Γₚₗ, Γₚᵣ, Γₛₗ, Γₛᵣ) := match i with
+    | .p i => (
+      Γₚ |>.eraseIdxR i |>.concat P1, Γₚ |>.eraseIdxR i |>.concat P2,
+      Γₛ, Γₛ)
+    | .s i => (
+      Γₚ, Γₚ,
+      Γₛ |>.eraseIdxR i |>.concat P1, Γₛ |>.eraseIdxR i |>.concat P2)
+  envs_entails ⟨Γₚₗ, Γₛₗ⟩ Q →
+  envs_entails ⟨Γₚᵣ, Γₛᵣ⟩ Q →
+  envs_entails ⟨Γₚ, Γₛ⟩ Q
 := sorry
 
 end Iris.Proofmode
