git/larsk21/iris-lean/src/Iris/Tests/Tactics.lean
@@ -1,0 +1,407 @@
+import Iris.BI
+import Iris.Proofmode
+
+namespace Iris.Tests
+open Iris.BI
+
+-- start stop
+theorem startStop [BI PROP] (Q : PROP) (H : Q ⊢ Q) : Q ⊢ Q := by
+  istart_proof
+  iintro HQ
+  istop_proof
+  exact H
+
+-- rename
+namespace rename
+
+theorem rename [BI PROP] (Q : PROP) : Q ⊢ Q := by
+  iintro HQ
+  irename HQ into H
+  iexact H
+
+theorem renameTwice [BI PROP] (Q : PROP) : Q ⊢ Q := by
+  iintro HQ
+  irename HQ into H
+  irename H into HQ
+  iexact HQ
+
+theorem renameId [BI PROP] (Q : PROP) : Q ⊢ Q := by
+  iintro HQ
+  irename HQ into HQ
+  iexact HQ
+
+end rename
+
+-- clear
+namespace clear
+
+theorem intuitionistic [BI PROP] (Q : PROP) : □ P ⊢ Q -∗ Q := by
+  iintro #HP
+  iintro HQ
+  iclear HP
+  iexact HQ
+
+theorem ispatial [BI PROP] (Q : PROP) : <affine> P ⊢ Q -∗ Q := by
+  iintro HP
+  iintro HQ
+  iclear HP
+  iexact HQ
+
+end clear
+
+-- intro
+namespace intro
+
+theorem spatial [BI PROP] (Q : PROP) : Q ⊢ Q := by
+  iintro HQ
+  iexact HQ
+
+theorem intuitionistic [BI PROP] (Q : PROP) : □ Q ⊢ Q := by
+  iintro #HQ
+  iexact HQ
+
+theorem drop [BI PROP] (Q : PROP) : ⊢ (P → Q -∗ Q) := by
+  iintro _ HQ
+  iexact HQ
+
+theorem dropAfter [BI PROP] (Q : PROP) : ⊢ Q -∗ (P → Q) := by
+  iintro HQ _
+  iexact HQ
+
+theorem «forall» [BI PROP] : ⊢ ∀ x, (⌜x = 0⌝ → ⌜x = 0⌝ : PROP) := by
+  iintro %x
+  iintro H
+  iexact H
+
+theorem pure [BIAffine PROP] (Q : PROP) : ⊢ ⌜φ⌝ -∗ Q -∗ Q := by
+  iintro %Hφ HQ
+  iexact HQ
+
+theorem pattern [BI PROP] (Q : PROP) : □ (P1 ∨ P2) ∗ Q ⊢ Q := by
+  iintro ⟨#(HP1 | HP2), HQ⟩
+  <;> iexact HQ
+
+theorem multipleSpatial [BI PROP] (Q : PROP) : ⊢ <affine> P -∗ Q -∗ Q := by
+  iintro HP HQ
+  iexact HQ
+
+theorem multipleIntuitionistic [BI PROP] (Q : PROP) : ⊢ □ P -∗ □ Q -∗ Q := by
+  iintro #HP #HQ
+  iexact HQ
+
+theorem multiplePatterns [BI PROP] (Q : PROP) : ⊢ □ (P1 ∧ P2) -∗ Q ∨ Q -∗ Q := by
+  iintro #⟨HP1, -#HP2⟩ (HQ | HQ)
+  <;> iexact HQ
+
+end intro
+
+-- exact
+namespace exact
+
+theorem exact [BI PROP] (Q : PROP) : Q ⊢ Q := by
+  iintro HQ
+  iexact HQ
+
+theorem defEq [BI PROP] (Q : PROP) : <affine> <pers> Q ⊢ □ Q := by
+  iintro HQ
+  iexact HQ
+
+theorem intuitionistic [BI PROP] (Q : PROP) : □ Q ⊢ Q := by
+  iintro HQ
+  iexact HQ
+
+end exact
+
+-- assumption
+namespace assumption
+
+theorem exact [BI PROP] (Q : PROP) : Q ⊢ Q := by
+  iintro HQ
+  iassumption
+
+theorem fromAssumption [BI PROP] (Q : PROP) : <affine> <pers> Q ⊢ □ Q := by
+  iintro HQ
+  iassumption
+
+theorem intuitionistic [BI PROP] (Q : PROP) : □ Q ⊢ Q := by
+  iintro #HQ
+  iassumption
+
+theorem lean [BI PROP] (Q : PROP) (H : ⊢ Q) : <affine> P ⊢ Q := by
+  iintro HP
+  iassumption
+
+theorem false [BI PROP] (Q : PROP) : False ⊢ Q := by
+  iintro H
+  iassumption
+
+end assumption
+
+-- pure
+namespace pure
+
+theorem move [BI PROP] (Q : PROP) : <affine> ⌜φ⌝ ⊢ Q -∗ Q := by
+  iintro Hφ
+  iintro HQ
+  ipure Hφ
+  iexact HQ
+
+theorem moveMultiple [BI PROP] (Q : PROP) : <affine> ⌜φ1⌝ ⊢ <affine> ⌜φ2⌝ -∗ Q -∗ Q := by
+  iintro Hφ1
+  iintro Hφ2
+  iintro HQ
+  ipure Hφ1
+  ipure Hφ2
+  iexact HQ
+
+theorem moveConjunction [BI PROP] (Q : PROP) : (⌜φ1⌝ ∧ <affine> ⌜φ2⌝) ⊢ Q -∗ Q := by
+  iintro Hφ
+  iintro HQ
+  ipure Hφ
+  iexact HQ
+
+end pure
+
+-- intuitionistic
+namespace intuitionistic
+
+theorem move [BI PROP] (P : PROP) : □ P ⊢ Q -∗ Q := by
+  iintro HP
+  iintro HQ
+  iintuitionistic HP
+  iexact HQ
+
+theorem moveMultiple [BI PROP] (P : PROP) : □ P ⊢ □ Q -∗ Q := by
+  iintro HP
+  iintro HQ
+  iintuitionistic HP
+  iintuitionistic HQ
+  iexact HQ
+
+theorem moveTwice [BI PROP] (P : PROP) : □ P ⊢ Q -∗ Q := by
+  iintro HP
+  iintro HQ
+  iintuitionistic HP
+  iintuitionistic HP
+  iexact HQ
+
+end intuitionistic
+
+-- spatial
+namespace spatial
+
+theorem move [BI PROP] (P : PROP) : □ P ⊢ □ Q -∗ Q := by
+  iintro #HP
+  iintro #HQ
+  ispatial HP
+  iexact HQ
+
+theorem moveMultiple [BI PROP] (P : PROP) : □ P ⊢ □ Q -∗ Q := by
+  iintro #HP
+  iintro #HQ
+  ispatial HP
+  ispatial HQ
+  iexact HQ
+
+theorem moveTwice [BI PROP] (P : PROP) : □ P ⊢ □ Q -∗ Q := by
+  iintro #HP
+  iintro #HQ
+  ispatial HP
+  ispatial HP
+  iexact HQ
+
+end spatial
+
+-- split
+namespace split
+
+theorem and [BI PROP] (Q : PROP) : Q ⊢ Q ∧ Q := by
+  iintro HQ
+  isplit
+  <;> iexact HQ
+
+theorem sepLeft [BIAffine PROP] (Q : PROP) : ⊢ P -∗ Q -∗ R -∗ P ∗ Q := by
+  iintro HP
+  iintro HQ
+  iintro HR
+  isplit l [HP]
+  · iexact HP
+  · iexact HQ
+
+theorem sepRight [BIAffine PROP] (Q : PROP) : ⊢ P -∗ Q -∗ R -∗ P ∗ Q := by
+  iintro HP
+  iintro HQ
+  iintro HR
+  isplit r [HQ]
+  · iexact HP
+  · iexact HQ
+
+theorem sepLeftAll [BIAffine PROP] (Q : PROP) : ⊢ P -∗ □ Q -∗ R -∗ P ∗ Q := by
+  iintro HP
+  iintro #HQ
+  iintro HR
+  isplit l
+  · iexact HP
+  · iexact HQ
+
+theorem sepRightAll [BIAffine PROP] (Q : PROP) : ⊢ □ P -∗ Q -∗ R -∗ P ∗ Q := by
+  iintro #HP
+  iintro HQ
+  iintro HR
+  isplit r
+  · iexact HP
+  · iexact HQ
+
+end split
+
+-- cases
+namespace cases
+
+theorem rename [BI PROP] (P : PROP) : P ⊢ P := by
+  iintro HP
+  icases HP with H
+  iexact H
+
+theorem clear [BI PROP] (P Q : PROP) : ⊢ P -∗ <affine> Q -∗ P := by
+  iintro HP
+  iintro HQ
+  icases HQ with _
+  iexact HP
+
+theorem and [BI PROP] (Q : PROP) : □ (P1 ∧ P2 ∧ Q) ⊢ Q := by
+  iintro #HP
+  icases HP with ⟨HP1, HP2, HQ⟩
+  iexact HQ
+
+theorem andIntuitionistic [BI PROP] (Q : PROP) : □ P ∧ Q ⊢ Q := by
+  iintro HPQ
+  icases HPQ with ⟨HP, HQ⟩
+  iexact HQ
+
+theorem andPersistentLeft [BI PROP] (Q : PROP) : <pers> Q ∧ <affine> P ⊢ Q := by
+  iintro HQP
+  icases HQP with ⟨#HQ, HP⟩
+  iexact HQ
+
+theorem andPersistentRight [BI PROP] (Q : PROP) : Q ∧ <pers> P ⊢ Q := by
+  iintro HQP
+  icases HQP with ⟨HQ, HP⟩
+  iexact HQ
+
+theorem sep [BIAffine PROP] (Q : PROP) : P1 ∗ P2 ∗ Q ⊢ Q := by
+  iintro HPQ
+  icases HPQ with ⟨HP1, HP2, HQ⟩
+  iexact HQ
+
+theorem disjunction [BI PROP] (Q : PROP) : Q ⊢ <affine> (P1 ∨ P2 ∨ P3) -∗ Q := by
+  iintro HQ
+  iintro HP
+  icases HP with (HP1 | HP2 | HP3)
+  <;> iexact HQ
+
+theorem conjunctionAndDisjunction [BIAffine PROP] (Q : PROP) : (P11 ∨ P12 ∨ P13) ∗ P2 ∗ (P31 ∨ P32 ∨ P33) ∗ Q ⊢ Q := by
+  iintro HP
+  icases HP with ⟨HP11 | HP12 | HP13, HP2, HP31 | HP32 | HP33, HQ⟩
+  <;> iexact HQ
+
+theorem moveToPure [BI PROP] (Q : PROP) : ⊢ <affine> ⌜φ⌝ -∗ Q -∗ Q := by
+  iintro Hφ
+  iintro HQ
+  icases Hφ with %Hφ
+  iexact HQ
+
+theorem moveToIntuitionistic [BI PROP] (Q : PROP) : ⊢ □ Q -∗ Q := by
+  iintro HQ
+  icases HQ with #HQ
+  iexact HQ
+
+theorem moveToSpatial [BI PROP] (Q : PROP) : ⊢ □ Q -∗ Q := by
+  iintro #HQ
+  icases HQ with -#HQ
+  iexact HQ
+
+theorem moveToPureConjunction [BI PROP] (Q : PROP) : ⊢ <affine> ⌜φ⌝ ∗ Q -∗ Q := by
+  iintro HφQ
+  icases HφQ with ⟨%Hφ, HQ⟩
+  iexact HQ
+
+theorem moveToPureDisjunction [BI PROP] (Q : PROP) : ⊢ <affine> ⌜φ1⌝ ∨ <affine> ⌜φ2⌝ -∗ Q -∗ Q := by
+  iintro Hφ
+  iintro HQ
+  icases Hφ with (%Hφ1 | %Hφ2)
+  <;> iexact HQ
+
+theorem moveToIntuitionisticConjunction [BI PROP] (Q : PROP) : ⊢ □ P ∗ Q -∗ Q := by
+  iintro HPQ
+  icases HPQ with ⟨#HP, HQ⟩
+  iexact HQ
+
+theorem moveToIntuitionisticDisjunction [BI PROP] (Q : PROP) : ⊢ □ Q ∨ Q -∗ Q := by
+  iintro HQQ
+  icases HQQ with (#HQ | HQ)
+  <;> iexact HQ
+
+theorem moveToSpatialConjunction [BI PROP] (Q : PROP) : ⊢ □ (P ∧ Q) -∗ Q := by
+  iintro #HPQ
+  icases HPQ with ⟨HP, -#HQ⟩
+  iexact HQ
+
+theorem moveToSpatialDisjunction [BI PROP] (Q : PROP) : ⊢ □ (Q ∨ Q) -∗ Q := by
+  iintro #HPQ
+  icases HPQ with (HQ | -#HQ)
+  <;> iexact HQ
+
+theorem moveToIntuitionisticAndBackConjunction [BI PROP] (Q : PROP) : ⊢ □ (P ∧ Q) -∗ Q := by
+  iintro HPQ
+  icases HPQ with #⟨HP, -#HQ⟩
+  iexact HQ
+
+theorem moveToIntuitionisticAndBackDisjunction [BI PROP] (Q : PROP) : ⊢ □ (Q ∨ Q) -∗ Q := by
+  iintro HPQ
+  icases HPQ with #(HQ | -#HQ)
+  <;> iexact HQ
+
+theorem conjunctionClear [BIAffine PROP] (Q : PROP) : Q ∗ P ⊢ Q := by
+  iintro HQP
+  icases HQP with ⟨HQ, _⟩
+  <;> iexact HQ
+
+theorem disjunctionClear [BIAffine PROP] (Q : PROP) : Q ⊢ P1 ∨ P2 -∗ Q := by
+  iintro HQ
+  iintro HP
+  icases HP with (_ | HP2)
+  <;> iexact HQ
+
+theorem andDestructSpatialRight [BI PROP] (Q : PROP) : P ∧ Q ⊢ Q := by
+  iintro HPQ
+  icases HPQ with ⟨_, HQ⟩
+  iexact HQ
+
+theorem andDestructSpatialLeft [BI PROP] (Q : PROP) : Q ∧ P ⊢ Q := by
+  iintro HQP
+  icases HQP with ⟨HQ, _⟩
+  iexact HQ
+
+theorem andClearSpatialMultiple [BI PROP] (Q : PROP) : P1 ∧ P2 ∧ Q ∧ P3 ⊢ Q := by
+  iintro HPQ
+  icases HPQ with ⟨_, _, HQ, _⟩
+  iexact HQ
+
+theorem andDestructIntuitionisticRight [BI PROP] (Q : PROP) : □ (P ∧ Q) ⊢ Q := by
+  iintro #HPQ
+  icases HPQ with ⟨_, HQ⟩
+  iexact HQ
+
+theorem andDestructIntuitionisticLeft [BI PROP] (Q : PROP) : □ (Q ∧ P) ⊢ Q := by
+  iintro #HQP
+  icases HQP with ⟨HQ, _⟩
+  iexact HQ
+
+theorem andClearIntuitionisticMultiple [BI PROP] (Q : PROP) : □ (P1 ∧ P2 ∧ Q ∧ P3) ⊢ Q := by
+  iintro #HPQ
+  icases HPQ with ⟨_, _, HQ, _⟩
+  iexact HQ
+
+end cases
+
+end Iris.Tests
