git/user7230724/lean-projects4/Src/Prover/Func.lean
@@ -1,0 +1,30 @@
+import Src.Prover.Pair
+
+namespace prover
+noncomputable section
+
+def fn (A : Set) (f : Set → Set) : Set :=
+image A # λ b => pair b (f b)
+
+section open Lean
+macro "FN " "(" a:explicitBinders "∈" b:term ")" "," f:term : term =>
+expandExplicitBinders ``id a f >>= λ v => `(fn $b $v) end
+
+def app (f a : Set) : Set :=
+someu # λ b => pair a b ∈ f
+
+infixl:100 (priority := high) " ~ " => app
+
+theorem exiu_fn_ret {A : Set} {f : Set → Set} {a : Set} (h : a ∈ A) :
+  ∃! b, pair a b ∈ FN (x ∈ A), f x :=
+exiu_intro (f a) (mpr mem_image # exi_intro a # and_intro h rfl)
+(λ b h₁ => exi_elim (mp mem_image h₁) # λ c h₂ =>
+and_elim (mp pair_ext # and_right h₂) # λ h₃ h₄ =>
+eq_rec (λ x => b = f x) h₃ # eq_symm h₄)
+
+theorem fn_app {A : Set} {f : Set → Set} {a : Set} (h : a ∈ A) :
+  (FN (x ∈ A), f x) ~ a = f a :=
+hv (@someu_spec _ _ (λ b => pair a b ∈ FN (x ∈ A), f x) # exiu_fn_ret h) #
+λ h₁ => exi_elim (mp mem_image h₁) # λ x h₂ =>
+and_elim (mp pair_ext # and_right h₂) # λ h₃ h₄ =>
+eq_rec (λ x => fn A f ~ a = f x) h₃ # eq_symm h₄
